feat: WType'.uniform

Logic/Vorspiel/Computability.lean
@@ -14,6 +14,14 @@ def predO : ℕ → Option ℕ
 
 end Nat
 
+namespace List
+
+def range2 (n m : ℕ) : List (ℕ × ℕ) := (·, ·) <$> range n <*> range m
+
+@[simp] lemma mem_range2_iff {n m i j : ℕ} : (i, j) ∈ range2 n m ↔ i < n ∧ j < m := by simp[range2, seq_eq_bind]
+
+end List
+
 namespace Encodable
 
 variable {α : Type _} [Encodable α]
@@ -24,6 +32,11 @@ lemma encodeDecode_of_none {e : ℕ} (h : decode (α := α) e = none) : encodeDe
 
 lemma encodeDecode_of_some {e : ℕ} {a : α} (h : decode e = some a) : encodeDecode α e = some (encode a) := by simp[encodeDecode, h]
 
+lemma decode_encodeDecode : encodeDecode α e = some i → ∃ a : α, decode i = some a := by
+  simp[encodeDecode]
+  cases h : (decode e : Option α) <;> simp
+  rintro rfl; simp
+
 variable {α : Type u_1} {P : α → Prop} [Encodable α] [DecidablePred P]
 
 lemma encode_decode_subtype (e : ℕ) :
@@ -31,9 +44,107 @@ lemma encode_decode_subtype (e : ℕ) :
   rcases h : decode (α := α) e with (_ | s) <;> simp[*, decode, decodeSubtype, encode, encodeSubtype]
   { by_cases hs : P s <;> simp[hs] }
 
+lemma encodeDecode_subtype' (e : ℕ) :
+    encodeDecode {x // P x} e = (decode (α := α) e).bind (fun a => if P a then some (encode a) else none) := by
+  simp[encodeDecode, encode_decode_subtype]
+  rcases h : (decode e : Option α) with (_ | a) <;> simp
+  { by_cases ha : P a <;> simp[*] }
+
+lemma encodeDecode_subtype (e : ℕ) :
+    encodeDecode {x // P x} e = (encodeDecode α e).bind (fun c => if ∃ a ∈ (decode c : Option α), P a then some c else none) := by
+  simp[encodeDecode_subtype', encodeDecode]
+  rcases (decode e : Option α) <;> simp
+
+-- todo: delete
+lemma encode_decode_ofEquiv {β} (e : β ≃ α) (n : ℕ) :
+    haveI : Encodable β := Encodable.ofEquiv α e
+    encode (decode (α := β) n) = encode (decode (α := α) n) := by
+  simp[Encodable.decode_ofEquiv e]
+  rcases h : (decode n : Option α) with (_ | ⟨a⟩) <;> simp
+  { exact @Encodable.encode_none _ (Encodable.ofEquiv α e) }
+  { have := @Encodable.encode_some _ (Encodable.ofEquiv α e) (e.symm a); rw[this];
+    simpa using Encodable.encode_ofEquiv e (e.symm a) }
+
+-- todo: delete
+lemma encode_decode_ofEquiv_prim {α β} [Primcodable α] (e : β ≃ α) (n : ℕ) :
+    haveI : Primcodable β := Primcodable.ofEquiv α e
+    encode (decode (α := β) n) = encode (decode (α := α) n) := encode_decode_ofEquiv e n
+
+lemma encodeDecode_ofEquiv {β} (e : β ≃ α) :
+    haveI : Encodable β := Encodable.ofEquiv α e
+    encodeDecode β = encodeDecode α := by
+  funext n; simp[encodeDecode, Encodable.decode_ofEquiv e]
+  rcases h : (decode n : Option α) with (_ | ⟨a⟩) <;> simp
+  { simp[@Encodable.encode_none _ (Encodable.ofEquiv α e)] }
+  { have := @Encodable.encode_some _ (Encodable.ofEquiv α e) (e.symm a); rw[this];
+    simpa using Encodable.encode_ofEquiv e (e.symm a) } 
+
+lemma encode_decode_eq_encodeDecode : encode (decode e : Option α) = encode (encodeDecode α e) := by
+  simp[encodeDecode]; cases (decode e : Option α) <;> simp
+
+lemma encode_decode_sigma_s {β : α → Type _} [(a : α) → Encodable (β a)] {e : ℕ} :
+    encodeDecode ((a : α) × β a) e = ((decode e.unpair.1 : Option α).bind $ fun a => (encodeDecode (β a) e.unpair.2).map $ fun b => (encode a).pair b) := by
+  rcases ha : (decode e.unpair.1 : Option α) with (_ | a) <;> simp[*, encodeDecode]
+  { rcases (decode e.unpair.2 : Option (β a)) with (_ | b) <;> simp[*] }
+
+lemma encode_decode_sigma_of_none {β : α → Type _} [(a : α) → Encodable (β a)] {e : ℕ} (h : (decode e.unpair.1 : Option α) = none) :
+    encodeDecode (α := (a : α) × β a) e = none := by
+  simp[encodeDecode, h]
+
+lemma encode_decode_sigma_of_some {β : α → Type _} [(a : α) → Encodable (β a)] {e : ℕ} {a : α} (h : decode e.unpair.1 = some a) :
+    encodeDecode ((a : α) × β a) e = (encodeDecode (β a) e.unpair.2).map fun b => (encode a).pair b := by
+  simp[encodeDecode, h]; rcases h : decode e.unpair.2 with (_ | b) <;> simp
+
 end Encodable
 
+namespace Primcodable
+
+open Encodable
+
+instance fintypeArrow [DecidableEq α] [Fintype α] [Encodable α] {β : Type _} [Primcodable β] : Primcodable (α → β) :=
+    Primcodable.ofEquiv (Fin (Fintype.card α) → β) (Equiv.arrowCongr Encodable.fintypeEquivFin (Equiv.refl _))
+
+lemma ofEquiv_toEncodable {α : Type _} {β : Type _} [Primcodable α] (e : β ≃ α) :
+  (ofEquiv α e).toEncodable = Encodable.ofEquiv α e := rfl
+
+end Primcodable
+
 namespace Primrec
+
+lemma nat_strong_rec' [Primcodable α] [Primcodable σ] (f : α → ℕ → σ) {g : α × ℕ → List σ → Option σ} (hg : Primrec₂ g)
+  (H : ∀ a n, g (a, n) ((List.range n).map (f a)) = some (f a n)) : Primrec₂ f := by
+  let g' : α → List σ → Option σ := fun a l => g (a, l.length) l
+  have : Primrec₂ g' := hg.comp₂ (pair fst (list_length.comp snd)) Primrec₂.right
+  exact nat_strong_rec f this (by simpa using H)
+
+lemma nat_strong_rec'2 [Primcodable α] [Primcodable σ] (f : α → ℕ × ℕ → σ) {g : α × (ℕ × ℕ) → List σ → Option σ} (hg : Primrec₂ g)
+  (H : ∀ a n m, g (a, (n, m)) ((List.range (n.pair m)).map (fun i => f a i.unpair)) = some (f a (n, m))) : Primrec₂ f := by
+  let g' : α × ℕ → List σ → Option σ := fun (a, n) => g (a, n.unpair)
+  have : Primrec₂ g' := hg.comp₂ (pair (fst.comp fst) (unpair.comp $ snd.comp fst)) Primrec₂.right
+  have : Primrec₂ (fun a n => f a n.unpair : α → ℕ → σ) := nat_strong_rec' (fun a n => f a n.unpair : α → ℕ → σ) this (fun a n => by simpa using H a n.unpair.1 n.unpair.2)
+  have : Primrec₂ (fun a p => (fun a n => f a n.unpair : α → ℕ → σ) a (p.1.pair p.2) : α → ℕ × ℕ → σ) :=
+    this.comp₂ Primrec₂.left (Primrec₂.natPair.comp (fst.comp snd) (snd.comp snd))
+  exact this.of_eq (by simp)
+
+lemma nat_strong_rec'2' [Primcodable σ] (f : ℕ → ℕ → σ) {g : ℕ × ℕ → List σ → Option σ} (hg : Primrec₂ g)
+  (H : ∀ n m, g (n, m) ((List.range (n.pair m)).map (fun i => f i.unpair.1 i.unpair.2)) = some (f n m)) : Primrec₂ f := by
+  have : Primrec₂ (fun p => g p.2 : Unit × (ℕ × ℕ) → List σ → Option σ) := hg.comp (snd.comp fst) snd
+  have := nat_strong_rec'2 (fun _ i => f i.1 i.2 : Unit → ℕ × ℕ → σ) this (by simpa using H)
+  have : Primrec₂ (fun n m => (fun _ i => f i.1 i.2 : Unit → ℕ × ℕ → σ) () (n, m)) := this.comp (const ()) Primrec.id
+  exact this.of_eq (by simp)
+
+lemma option_list_mapM' [Primcodable α] [Primcodable β] [Primcodable γ]
+  {f : α → List β} {g : α → β → Option γ} (hf : Primrec f) (hg : Primrec₂ g) : Primrec (fun a => (f a).mapM' (g a)) := by
+  have : Primrec₂ (fun a p => (g a p.1).bind $ fun c => p.2.2.map $ fun l => c :: l : α → β × List β × Option (List γ) → Option (List γ)) :=
+    Primrec.option_bind (hg.comp fst (fst.comp snd)) (Primrec.option_map (snd.comp $ snd.comp $ snd.comp fst) (Primrec.list_cons.comp₂ (snd.comp fst) Primrec₂.right))
+  let F : α → Option (List γ) := fun a => List.recOn (f a) (some []) (fun b _ ih => (g a b).bind $ fun c => ih.map $ fun l => c :: l)
+  have : Primrec F := Primrec.list_rec hf (const (some [] : Option (List γ))) this
+  have e : ∀ (k : β → Option γ) (bs : List β),
+    List.recOn bs (some [] : Option (List γ)) (fun b _ ih => (k b).bind $ fun c => ih.map $ fun l => c :: l) = bs.mapM' k := by
+    intro k bs
+    induction bs <;> simp[Option.pure_eq_some, Option.bind_eq_bind, *]
+    { simp[Option.map_eq_bind, Function.comp] }
+  exact this.of_eq (by simp[e])
 
 open Encodable
 variable {α : Type _} [Primcodable α]
@@ -41,15 +152,23 @@ variable {α : Type _} [Primcodable α]
 lemma nat_predO : Primrec Nat.predO :=
   (Primrec.nat_casesOn₁ none (Primrec.option_some_iff.mpr Primrec.id)).of_eq (by intro n; cases n <;> simp)
 
+protected lemma encodeDecode : Primrec (fun e => encodeDecode α e) := nat_predO.comp (Primrec.encode.comp Primrec.decode)
+
 class Uniform {α : Type u} (β : α → Type v) [Primcodable α] [∀ a, Primcodable (β a)] where
   uniformly_prim : Primrec₂ (fun a n => Encodable.encode (Encodable.decode (α := β a) n))
+
+class CardUniform {α : Type u} (β : α → Type v) [∀ a, Fintype (β a)] [Primcodable α] [∀ a, Primcodable (β a)] where
+  card_prim : Primrec fun a => Fintype.card (β a)
 
 namespace Uniform
 
 variable {α : Type u} {β γ : α → Type v} [Primcodable α] [(a : α) → Primcodable (β a)]
 
-lemma _root_.Primrec₂.encodeDecode [Uniform β] : Primrec₂ (fun a e => encodeDecode (β a) e) :=
+lemma _root_.Primrec₂.encodeDecode_u [Uniform β] : Primrec₂ (fun a e => encodeDecode (β a) e) :=
   (nat_predO.comp $ Uniform.uniformly_prim.comp fst snd)
+
+def ofEncodeDecode (h : Primrec₂ (fun a n => encodeDecode (β a) n)) : Uniform β where
+  uniformly_prim := (Primrec.encode.comp₂ h).of_eq (by simp[encode_decode_eq_encodeDecode])
 
 instance {β : Type _} [Primcodable β] : Uniform (Vector β) where
   uniformly_prim := by
@@ -74,6 +193,15 @@ instance {β : Type _} [Primcodable β] : Uniform (Fin · → β) where
         simpa using (this (Equiv.vectorEquivFin β n v)).symm }
     exact uniformly_prim.of_eq this
 
+instance fintypeArrow [DecidableEq α] [Fintype α] {β : Type _} [Primcodable β] : Primcodable (α → β) :=
+    Primcodable.ofEquiv (Fin (Fintype.card α) → β) (Equiv.arrowCongr fintypeEquivFin (Equiv.refl _))
+
+instance {γ : α → Type _} [(a : α) → Fintype (γ a)] [(a : α) → DecidableEq (γ a)] [(a : α) → Primcodable (γ a)] [CardUniform γ]
+  {β : Type _} [Primcodable β] : Uniform (γ · → β) where
+  uniformly_prim := by
+    simp[Encodable.encode_decode_ofEquiv_prim]
+    exact (Uniform.uniformly_prim (β := Vector β)).comp₂ (CardUniform.card_prim.comp fst) Primrec₂.right
+
 attribute [instance] Encodable.finPi
 
 instance : Uniform Fin where
@@ -95,9 +223,9 @@ instance {β : α → Type _} {γ : α → Type _} [(a : α) → Primcodable (β
     have : Primrec₂ (fun a e => encode ((encodeDecode (β a) e.unpair.1).bind $ fun b => (encodeDecode (γ a) e.unpair.2).map $ fun c => Nat.pair b c) : α → ℕ → ℕ) :=
       Primrec.encode.comp
         (Primrec.option_bind
-          (Primrec₂.encodeDecode.comp fst (fst.comp $ Primrec.unpair.comp $ snd))
+          (Primrec₂.encodeDecode_u.comp fst (fst.comp $ Primrec.unpair.comp $ snd))
           (Primrec.option_map
-            (Primrec₂.encodeDecode.comp (fst.comp $ fst) (snd.comp $ Primrec.unpair.comp $ snd.comp $ fst))
+            (Primrec₂.encodeDecode_u.comp (fst.comp $ fst) (snd.comp $ Primrec.unpair.comp $ snd.comp $ fst))
             (Primrec₂.natPair.comp₂ (snd.comp $ fst) Primrec₂.right)))
     exact this.of_eq e
 
@@ -120,9 +248,195 @@ instance sigma [Uniform β] : Primcodable (Sigma β) where
     have p₁ : Primrec (fun e => decode e.unpair.1 : ℕ → Option α) := (Primrec.decode.comp $ fst.comp $ Primrec.unpair)
     have p₂ : Primrec₂ (fun e a => (encodeDecode (β a) e.unpair.2).map (Nat.pair (encode a)) : ℕ → α → Option ℕ) :=
       (Primrec.option_map
-        (Primrec₂.encodeDecode.comp snd (snd.comp $ Primrec.unpair.comp $ fst))
+        (Primrec₂.encodeDecode_u.comp snd (snd.comp $ Primrec.unpair.comp $ fst))
         (Primrec₂.natPair.comp₂ (Primrec.encode.comp $ snd.comp $ fst) Primrec₂.right))
     exact Primrec.nat_iff.mp ((Primrec.encode.comp $ p₁.option_bind p₂).of_eq e)
 
+@[simp] lemma sigma_toEncodable_eq [Uniform β] : (sigma : Primcodable (Sigma β)).toEncodable = Sigma.encodable := rfl
+
 end Primrec
+
+namespace Encodable
+
+open Primcodable Primrec.Uniform
+attribute [-instance] Encodable.finPi Encodable.fintypeArrowOfEncodable
+
+lemma decode_list {β : Type _} [Encodable β] :
+    (e : ℕ) → (decode e : Option (List β)) = (Denumerable.ofNat (List ℕ) e).mapM' (decode : ℕ → Option β)
+  | 0     => by simp; rfl
+  | e + 1 =>
+    have : e.unpair.2 < e + 1 := Nat.lt_succ_of_le e.unpair_right_le
+    by  simp; rcases h : (decode e.unpair.1 : Option β) with (_ | b) <;> simp[seq_eq_bind, Option.bind_eq_bind]
+        have := decode_list (β := β) (e.unpair.2)
+        simp[this, Option.pure_eq_some, Option.map_eq_bind, Function.comp]
+
+lemma encodeDecode_list {β : Type _} [Encodable β] (e : ℕ) :
+    encodeDecode (List β) e = ((Denumerable.ofNat (List ℕ) e).mapM' (encodeDecode β : ℕ → Option ℕ)).map encode := by
+  simp[encodeDecode, decode_list]
+  generalize hr : (Denumerable.ofNat (List ℕ) e) = r
+  induction' r with rh rt ih generalizing e <;> simp[Option.pure_eq_some, Option.bind_eq_bind, Option.map_bind']
+  rcases hb : (decode rh) with (_ | b) <;> simp
+  rcases hbs : (mapM' decode rt) with (_ | bs) <;> simp
+  { have : mapM' (fun e => (encode (decode e : Option β)).predO) rt = none
+    { simp[encodeDecode, List.mapM'_eq_none_iff] at hbs ⊢
+      rcases hbs with ⟨a, ha, da⟩
+      exact ⟨a, ha, by simp[da]⟩  }
+    simp[this] }
+  { have ih : some (encode bs) = (mapM' (encodeDecode β) rt).map encode := by simpa[hbs] using ih (encode rt) (by simp)
+    suffices : some ((encode b).pair (encode bs) + 1) = ((mapM' (encodeDecode β) rt).map encode).map ((encode b).pair · + 1)
+    { simp[this]; simp[Option.map_eq_bind, Function.comp] }
+    simp[←ih] }
+
+lemma encodeDecode_finArrow {β : Type _} [Encodable β] {e : ℕ} :
+    encodeDecode (Fin k → β) e =
+    (((Denumerable.ofNat (List ℕ) e).mapM' (encodeDecode β)).bind $ fun l' => if l'.length = k then some (encode l') else none) := by
+  rw[encodeDecode_ofEquiv, encodeDecode_subtype, encodeDecode_list]; simp
+  rcases h : (mapM' (encodeDecode β) (Denumerable.ofNat (List ℕ) e)) with (_ | l) <;> simp
+  rcases hbs : decode (encode l) with (_ | bs)
+  { simp[decode_list] at hbs
+    have : ∃ a ∈ l, (decode a : Option β) = none := by simpa[List.mapM'_eq_none_iff] using hbs
+    rcases this with ⟨a, hal, ha⟩
+    have : ∃ a', encodeDecode β a' = some a := List.mapM'_mem_inversion h hal
+    rcases this with ⟨a', ha'⟩
+    simpa [ha] using decode_encodeDecode ha' }
+  { have : bs.length = l.length := by
+      simp[decode_list] at hbs; exact List.length_mapM' hbs
+    simp[this] }
+
+lemma encodeDecode_fintypeArrow (α : Type _) (β : Type _) [DecidableEq α] [Fintype α] [Primcodable α] [Primcodable β] (e : ℕ) :
+    encodeDecode (α → β) e =
+    (((Denumerable.ofNat (List ℕ) e).mapM' (encodeDecode β)).bind $ fun l' => if l'.length = Fintype.card α then some (encode l') else none) := by
+  simp[Primcodable.ofEquiv_toEncodable, fintypeArrow]; rw[encodeDecode_ofEquiv]
+  exact encodeDecode_finArrow (β := β)
+
+end Encodable
+
+namespace WType
+
+attribute [-instance] WType.instEncodableWType
+
+open Encodable Primrec
+variable {α : Type _} {β : α → Type _} [(a : α) → Fintype (β a)] [(a : α) → DecidableEq (β a)] [(a : α) → Primcodable (β a)] [Primcodable α] [Primrec.CardUniform β]
+
+@[reducible]
+private def WType' {α : Type _} (β : α → Type _) [(a : α) → Fintype (β a)] [(a : α) → Primcodable (β a)] (n : ℕ) :=
+  { t : WType β // t.depth ≤ n }
+
+def WType'.depth' : WType' β n → Fin (n + 1) := fun ⟨t, h⟩ => ⟨t.depth, Iff.mpr Nat.lt_succ h⟩
+
+def WType'.equiv_zero : WType' β 0 ≃ Empty where
+  toFun := fun ⟨x, h⟩ => False.elim (not_lt_of_ge h $ WType.depth_pos _)
+  invFun := by rintro ⟨⟩
+  left_inv := fun ⟨x, h⟩ => False.elim (not_lt_of_ge h $ WType.depth_pos _)
+  right_inv := by rintro ⟨⟩
+
+def WType'.equiv_succ : WType' β (n + 1) ≃ (Σ a : α, β a → WType' β n) where
+  toFun := fun ⟨t, h⟩ => by rcases t with ⟨a, f⟩; exact ⟨a, fun b => ⟨f b, by simp[WType.depth] at h; exact h b⟩⟩
+  invFun := fun ⟨a, f⟩ => ⟨WType.mk a (fun b => (f b).val), by simp[depth]; intro b; exact (f b).property⟩
+  left_inv := fun ⟨t, h⟩ => by rcases t with ⟨a, f⟩; simp
+  right_inv := fun ⟨a, f⟩ => by simp
+
+def WType'.primcodable_zero : Primcodable (WType' β 0) := Primcodable.ofEquiv _ WType'.equiv_zero
+
+def WType'.primcodable_succ (n) (i : Primcodable (WType' β n)) : Primcodable (WType' β (n + 1)) := Primcodable.ofEquiv _ WType'.equiv_succ
+
+instance WType'.primcodable (n : ℕ) : Primcodable (WType' β n) := Nat.rec WType'.primcodable_zero WType'.primcodable_succ n
+
+--instance : Encodable (WType β) := by
+--  haveI h' : ∀ n, Primcodable (WType' β n) := fun n => Nat.rec WType'.primcodable_zero WType'.primcodable_succ n
+--  let f : WType β → Σ n, WType' β n := fun t => ⟨t.depth, ⟨t, le_rfl⟩⟩
+--  let finv : (Σn, WType' β n) → WType β := fun p => p.2.1
+--  have : ∀ t, finv (f t) = t := fun t => rfl
+--  exact Encodable.ofLeftInverse f finv this
+
+attribute [-instance] Subtype.encodable Encodable.fintypeArrowOfEncodable
+
+lemma testeq {α : Type _} {a b c d : α} : a = b → b = c → c = d → a = d := by
+  intro hab hbc hcd; simp[hab, hbc, hcd]
+
+lemma WType'.encodeDecode_EType' (s e) :
+    encodeDecode (WType' β s) e =
+    Nat.casesOn s (encodeDecode (WType' β 0) e)
+      (fun s => (decode e.unpair.1 : Option α).bind
+        $ fun a => (((Denumerable.ofNat (List ℕ) e.unpair.2).mapM' (encodeDecode (WType' β s))).bind
+          $ fun l => if l.length = Fintype.card (β a) then some (encode l) else none).map
+            $ fun b => (encode a).pair b) := by
+  rcases s with (_ | s)
+  · simp
+  · have := Encodable.decode_sigma_val (γ := fun a => β a → WType' β s) e
+    simp[WType'.primcodable, primcodable_succ, Primcodable.ofEquiv_toEncodable]
+    rw[encodeDecode_ofEquiv equiv_succ, encode_decode_sigma_s]
+    rcases ha : (decode e.unpair.1 : Option α) with (_ | a)
+    · simp
+    · simp[encode_decode_ofEquiv, encodeDecode_fintypeArrow (β a) (WType' β s)]
+
+variable (β)
+
+private def strongRecE {γ : Type _} [Encodable γ] (zero : ℕ → γ) (succ : α → List γ → Option γ) : ℕ × ℕ → List (Option γ) → Option γ := fun (s, e) ih =>
+  Nat.casesOn s (zero e)
+    (fun s => (decode e.unpair.1 : Option α).bind
+      $ fun a => (((Denumerable.ofNat (List ℕ) e.unpair.2).mapM' (fun c => ih.getI (s.pair c))).bind
+        $ fun l => if l.length = Fintype.card (β a) then some l else none).bind
+          $ fun v => succ a v)
+
+@[reducible]
+private def g : ℕ × ℕ → List (Option ℕ) → Option ℕ := fun (s, e) ih =>
+  Nat.casesOn s (encodeDecode (WType' β 0) e)
+    (fun s => (decode e.unpair.1 : Option α).bind
+      $ fun a => (((Denumerable.ofNat (List ℕ) e.unpair.2).mapM' (fun c => ih.getI (s.pair c))).bind
+        $ fun l => if l.length = Fintype.card (β a) then some (encode l) else none).map
+          $ fun v => (encode a).pair v)
+
+variable {β}
+
+private lemma gh : g β (s, e) ((List.range (s.pair e)).map (fun i => encodeDecode (WType' β i.unpair.1) i.unpair.2)) = encodeDecode (WType' β s) e := by
+  simp[WType'.encodeDecode_EType' s e, g]
+  rcases s with (_ | s) <;> simp
+  have :
+    mapM' (fun c =>
+            List.getI
+              (List.map (fun i => encodeDecode (WType.WType' β i.unpair.1) i.unpair.2) (List.range ((s + 1).pair e)))
+            (s.pair c))
+          (Denumerable.ofNat (List ℕ) e.unpair.2) =
+    mapM' (encodeDecode (WType.WType' β s)) (Denumerable.ofNat (List ℕ) e.unpair.2) :=
+    List.mapM'_eq_mapM'_of_eq _ (by
+      { intro c hc
+        have : s.pair c < (s + 1).pair e := by
+          have : c < e.unpair.2 := Denumerable.lt_of_mem_list _ _ hc
+          exact lt_of_lt_of_le (Nat.pair_lt_pair_right s this) (Nat.pair_le_pair_of_le (Nat.le_succ s) (Nat.unpair_right_le e))
+        simp[List.getI_map_range _ this]; rw[Nat.unpair_pair s c] })
+  rw[this]
+
+/-
+-- 以下の証明はチェックに異常な時間がかかる（なぜ？）：
+example [Primcodable α] : Primrec₂ (fun a b => Nat.pair (Encodable.encode a.snd) b : (ℕ × ℕ × ℕ) × α → ℕ → ℕ) :=
+  Primrec₂.natPair.comp (Primrec.encode.comp (Primrec.snd.comp Primrec.fst)) Primrec.snd
+
+-- 以下はうまく行く
+example [Primcodable α] : Primrec₂ (fun a b => Nat.pair (Encodable.encode a.snd) b : (ℕ × ℕ × ℕ) × α → ℕ → ℕ) :=
+  by apply Primrec₂.natPair.comp (Primrec.encode.comp (Primrec.snd.comp Primrec.fst)) Primrec.snd
+-/
+
+private lemma g_primrec : Primrec₂ (g β) :=
+  have h₁ : Primrec₂ (fun a b => Nat.pair (encode a.snd) b : (((ℕ × ℕ) × List (Option ℕ)) × ℕ) × α → ℕ → ℕ) := by 
+    apply Primrec₂.natPair.comp (Primrec.encode.comp (snd.comp fst)) snd
+  have h₂ : Primrec₂ (fun a l => if l.length = Fintype.card (β a.snd) then some (encode l) else none
+    : (((ℕ × ℕ) × List (Option ℕ)) × ℕ) × α → List ℕ → Option ℕ) := by
+    apply Primrec.ite (Primrec.eq.comp (list_length.comp snd) (CardUniform.card_prim.comp $ snd.comp fst))
+      (Primrec.option_some.comp $ Primrec.encode.comp snd) (const none)
+  have h₃ : Primrec (fun a => mapM' (fun c => a.1.1.2.getI (a.1.2.pair c)) (Denumerable.ofNat (List ℕ) a.1.1.1.2.unpair.2)
+    : (((ℕ × ℕ) × List (Option ℕ)) × ℕ) × α → Option (List ℕ)) := by
+    apply option_list_mapM'
+      (by apply (Primrec.ofNat _).comp $ snd.comp $ Primrec.unpair.comp $ snd.comp $ fst.comp $ fst.comp $ fst)
+      (by apply Primrec.list_getI.comp (snd.comp $ fst.comp $ fst.comp $ fst) (Primrec₂.natPair.comp (snd.comp $ fst.comp fst) snd))
+  by apply Primrec.nat_casesOn (fst.comp fst) (Primrec.encodeDecode.comp (snd.comp fst))
+      (by apply
+            Primrec.option_bind (Primrec.decode.comp $ fst.comp $ Primrec.unpair.comp $ snd.comp $ fst.comp fst)
+            (by apply Primrec.option_map (by apply Primrec.option_bind (by apply h₃) (by apply h₂)) h₁))
+
+lemma WType'.uniform : Primrec.Uniform (WType' β) :=
+  have : Primrec₂ (fun p t => some (g β p t)) := option_some.comp g_primrec
+  Uniform.ofEncodeDecode (nat_strong_rec'2' _ this (by simp[gh]))
+
+end WType
 
